code/experimental/ed25519/Hacl.Impl.Ed25519.Sign.Steps.fst
@@ -223,26 +223,27 @@ let sign_step_2 signature secret msg len g tmp_bytes tmp_ints =
   let prefix_at_msg = Buffer.sub prefix_at_message 32ul FStar.UInt32.(32ul +^ len) in
   let message       = Buffer.sub prefix_at_msg 32ul len in
   let prefix'       = Buffer.sub prefix_at_msg 0ul 32ul in
-  lemma_sub len tmp_bytes';
-  let h0 = ST.get() in
-  copy_bytes prefix' prefix 32ul;
-  let h1 = ST.get() in
-  no_upd_lemma_1 h0 h1 prefix' message;
-  no_upd_lemma_1 h0 h1 prefix' a;
-  no_upd_lemma_1 h0 h1 prefix' a'';
-  lemma_append2 h1 prefix_at_msg 32ul len;
-  assert(as_seq h1 prefix' == as_seq h0 prefix);
-  assert(as_seq h1 message == as_seq h0 message);
-  assert(as_seq h1 prefix_at_msg == FStar.Seq.(as_seq h1 prefix' @| as_seq h1 message));
-  assert(as_seq h1 prefix_at_msg == FStar.Seq.(as_seq h0 prefix @| as_seq h0 msg));
-  assert(live h1 r);
-  assert(live h1 prefix_at_msg);
-  Hacl.Impl.SHA512.ModQ.sha512_modq r prefix_at_msg (len+^32ul);
-  let h2 = ST.get() in
-  no_upd_lemma_1 h1 h2 r message;
-  no_upd_lemma_1 h1 h2 r a;
-  no_upd_lemma_1 h1 h2 r a'';
-  ()
+  (* lemma_sub len tmp_bytes'; *)
+  (* let h0 = ST.get() in *)
+  (* copy_bytes prefix' prefix 32ul; *)
+  (* let h1 = ST.get() in *)
+  (* no_upd_lemma_1 h0 h1 prefix' message; *)
+  (* no_upd_lemma_1 h0 h1 prefix' a; *)
+  (* no_upd_lemma_1 h0 h1 prefix' a''; *)
+  (* lemma_append2 h1 prefix_at_msg 32ul len; *)
+  (* assert(as_seq h1 prefix' == as_seq h0 prefix); *)
+  (* assert(as_seq h1 message == as_seq h0 message); *)
+  (* assert(as_seq h1 prefix_at_msg == FStar.Seq.(as_seq h1 prefix' @| as_seq h1 message)); *)
+  (* assert(as_seq h1 prefix_at_msg == FStar.Seq.(as_seq h0 prefix @| as_seq h0 msg)); *)
+  (* assert(live h1 r); *)
+  (* assert(live h1 prefix_at_msg); *)
+  (* Hacl.Impl.SHA512.ModQ.sha512_modq r prefix_at_msg (len+^32ul); *)
+  Hacl.Impl.SHA512.ModQ.sha512_modq_pre r prefix msg len
+  (* let h2 = ST.get() in *)
+  (* no_upd_lemma_1 h1 h2 r message; *)
+  (* no_upd_lemma_1 h1 h2 r a; *)
+  (* no_upd_lemma_1 h1 h2 r a''; *)
+  (* () *)
 
 
 #reset-options "--max_fuel 0 --z3rlimit 50"
@@ -336,19 +337,20 @@ let sign_step_4 signature secret msg len g tmp_bytes tmp_ints =
   let rs_bytes = Buffer.sub prefix_at_message 0ul  32ul in
   let a_bytes  = Buffer.sub prefix_at_message 32ul 32ul in
   let message = Buffer.sub prefix_at_message 64ul len in
-  lemma_sub len tmp_bytes';
-  let h0 = ST.get() in
-  assume(as_seq h0 (Buffer.sub prefix_at_message 64ul len) == as_seq h0 msg);
-  append_before_sha msg len prefix_at_message rs' a'';
-  let h1 = ST.get() in
-  no_upd_lemma_1 h0 h1 prefix_at_message a;
-  no_upd_lemma_1 h0 h1 prefix_at_message rs';
-  no_upd_lemma_1 h0 h1 prefix_at_message r;
-  Hacl.Impl.SHA512.ModQ.sha512_modq h prefix_at_message (len+^64ul);
-  let h2 = ST.get() in
-  no_upd_lemma_1 h1 h2 h a;
-  no_upd_lemma_1 h1 h2 h rs';
-  no_upd_lemma_1 h1 h2 h r
+  (* lemma_sub len tmp_bytes'; *)
+  (* let h0 = ST.get() in *)
+  (* assume(as_seq h0 (Buffer.sub prefix_at_message 64ul len) == as_seq h0 msg); *)
+  (* append_before_sha msg len prefix_at_message rs' a''; *)
+  (* let h1 = ST.get() in *)
+  (* no_upd_lemma_1 h0 h1 prefix_at_message a; *)
+  (* no_upd_lemma_1 h0 h1 prefix_at_message rs'; *)
+  (* no_upd_lemma_1 h0 h1 prefix_at_message r; *)
+  (* Hacl.Impl.SHA512.ModQ.sha512_modq h prefix_at_message (len+^64ul); *)
+  Hacl.Impl.SHA512.ModQ.sha512_modq_pre_pre2 h rs' a'' msg len
+  (* let h2 = ST.get() in *)
+  (* no_upd_lemma_1 h1 h2 h a; *)
+  (* no_upd_lemma_1 h1 h2 h rs'; *)
+  (* no_upd_lemma_1 h1 h2 h r *)
 
 
 #reset-options "--max_fuel 0 --z3rlimit 20"
@@ -471,164 +473,3 @@ let sign_step_5 signature secret msg len g tmp_bytes tmp_ints =
   Hacl.Impl.BignumQ.Mul.add_modq s r ha;
   Hacl.Impl.Store56.store_56 s' s
 
-  (* copy_bytes (Buffer.sub signature 0ul 32ul) rs' 32ul; *)
-  (* copy_bytes (Buffer.sub signature 32ul 32ul) s' 32ul; *)
-  (* let h'' = ST.get() in *)
-  (* lemma_append2 h'' signature 32ul 32ul; *)
-  (* admit(); *)
-  (* (\* blit rs' 0ul signature 0ul 32ul; *\) *)
-  (* (\* blit s' 0ul signature 32ul 32ul; *\) *)
-  (* pop_frame() *)
-
-
-
-(* [@ "substitute"] *)
-(* private *)
-(* val sign__: *)
-(*   signature:hint8_p{length signature = 64} -> *)
-(*   secret:hint8_p{length secret = 32} -> *)
-(*   msg:hint8_p{length msg < pow2 32 - 64} -> *)
-(*   len:UInt32.t{UInt32.v len = length msg} -> *)
-(*   g:point -> *)
-(*   tmp_bytes:hint8_p{length tmp_bytes = 352 + UInt32.v len} -> *)
-(*   tmp_ints:buffer Hacl.UInt64.t{length tmp_ints = 65} -> *)
-(*   Stack unit *)
-(*     (requires (fun h -> live h signature /\ live h msg /\ live h secret /\ live h g /\  *)
-(*       live h tmp_bytes /\ live h tmp_ints /\ as_point h g == Spec.Ed25519.g /\ *)
-(*       as_seq h (Buffer.sub tmp_bytes 64ul len) == as_seq h msg)) *)
-(*     (ensures (fun h0 _ h1 -> live h0 signature /\ live h0 msg /\ live h0 secret /\ *)
-(*       live h1 signature /\ modifies_3 signature tmp_bytes tmp_ints h0 h1 /\ *)
-(*       h1.[signature] == Spec.Ed25519.sign h0.[secret] h0.[msg])) *)
-
-
-(* #reset-options "--max_fuel 0 --z3rlimit 200" *)
-
-(* let sign__ signature secret msg len g tmp_bytes tmp_ints = *)
-(*   (\* push_frame(); *\) *)
-(*   let tmpa = Buffer.sub tmp_ints 0ul  20ul in *)
-(*   let r    = Buffer.sub tmp_ints 20ul 5ul  in *)
-(*   let r'   = Buffer.sub tmp_ints 25ul 20ul in *)
-(*   let aq   = Buffer.sub tmp_ints 45ul 5ul  in *)
-(*   let ha   = Buffer.sub tmp_ints 50ul 5ul  in *)
-(*   let s    = Buffer.sub tmp_ints 55ul 5ul  in *)
-(*   let h    = Buffer.sub tmp_ints 60ul 5ul  in *)
-(*   let prefix_at_message = Buffer.sub tmp_bytes 0ul FStar.UInt32.(64ul +^ len) in *)
-(*   let tmp_bytes         = Buffer.offset tmp_bytes FStar.UInt32.(64ul +^ len) in *)
-(*   let buf  = Buffer.sub tmp_bytes 0ul   96ul in *)
-(*   let a''  = Buffer.sub tmp_bytes 96ul  32ul in *)
-(*   let rb   = Buffer.sub tmp_bytes 128ul 32ul in *)
-(*   let rs'  = Buffer.sub tmp_bytes 160ul 32ul in *)
-(*   let s'   = Buffer.sub tmp_bytes 192ul 32ul in *)
-(*   let apre = Buffer.sub tmp_bytes 224ul 64ul in *)
-(*   (\* Hacl.Impl.Ed25519.SecretExpand.secret_expand apre secret; *\) *)
-(*   (\* let a      = Buffer.sub apre 0ul 32ul in *\) *)
-(*   (\* let prefix = Buffer.sub apre 32ul 64ul in *\) *)
-(*   (\* point_mul_compress a'' a g; *\) *)
-(*   sign_step_1 signature secret msg len g tmp_bytes tmp_ints; *)
-(*   (\* TODO: use an incremental version of SHA instead so as to minimize *)
-(*   the copies and enable compilation with CompCert *\) *)
-
-(*   (\* let prefix_at_msg = Buffer.sub prefix_at_message 32ul FStar.UInt32.(32ul +^ len) in *\) *)
-(*   (\* let message       = Buffer.sub prefix_at_msg 32ul len in *\) *)
-(*   (\* let prefix'       = Buffer.sub prefix_at_msg 0ul 32ul in *\) *)
-(*   (\* copy_bytes prefix' prefix 32ul; *\) *)
-(*   (\* let h0 = ST.get() in *\) *)
-(*   (\* lemma_append2 h0 prefix_at_msg 32ul len; *\) *)
-(*   (\* Hacl.Impl.SHA512.ModQ.sha512_modq r prefix_at_msg (len+^32ul); *\) *)
-(*   sign_step_2 signature secret msg len g tmp_bytes tmp_ints; *)
-
-
-(*   sign_step_3 signature secret msg len g tmp_bytes tmp_ints; *)
-
-(*   (\* Hacl.Impl.Store56.store_56 rb r; *\) *)
-(*   (\* point_mul_compress rs' rb g; *\) *)
-(*   (\* Hacl.Impl.Ed25519.Ladder.point_mul r' rb g; *\) *)
-(*   (\* Hacl.Impl.Ed25519.PointCompress.point_compress rs' r'; *\) *)
-
-(*   (\* let rs_bytes = Buffer.sub prefix_at_message 0ul  32ul in *\) *)
-(*   (\* let a_bytes  = Buffer.sub prefix_at_message 32ul 32ul in *\) *)
-(*   (\* copy_bytes rs_bytes rs' 32ul; *\) *)
-(*   (\* copy_bytes a_bytes a'' 32ul; *\) *)
-(*   (\* (\\* blit rs'  0ul prefix_at_message 0ul 32ul; *\\) *\) *)
-(*   (\* (\\* blit a''  0ul prefix_at_message 32ul 32ul; *\\) *\) *)
-(*   (\* let h' = ST.get() in *\) *)
-(*   (\* lemma_append h' prefix_at_message 32ul 32ul len; *\) *)
-(*   (\* Hacl.Impl.SHA512.ModQ.sha512_modq h prefix_at_message (len+^64ul); *\) *)
-
-(*   sign_step_3 signature secret msg len g tmp_bytes tmp_ints; *)
-
-(*   sign_step_4 signature secret msg len g tmp_bytes tmp_ints; *)
-
-(*   (\* Hacl.Impl.Load56.load_32_bytes aq a; *\) *)
-(*   (\* Hacl.Impl.BignumQ.Mul.mul_modq ha h aq; *\) *)
-(*   (\* Hacl.Impl.BignumQ.Mul.add_modq s r ha; *\) *)
-(*   (\* Hacl.Impl.Store56.store_56 s' s; *\) *)
-
-(*   copy_bytes (Buffer.sub signature 0ul 32ul) rs' 32ul; *)
-(*   copy_bytes (Buffer.sub signature 32ul 32ul) s' 32ul; *)
-(*   let h'' = ST.get() in *)
-(*   lemma_append2 h'' signature 32ul 32ul; *)
-(*   () *)
-(*   (\* pop_frame() *\) *)
-
-
-(* #reset-options "--max_fuel 0 --z3rlimit 20" *)
-
-(* val sign_: *)
-(*   signature:hint8_p{length signature = 64} -> *)
-(*   secret:hint8_p{length secret = 32} -> *)
-(*   msg:hint8_p{length msg < pow2 32 - 64} -> *)
-(*   len:UInt32.t{UInt32.v len = length msg /\ UInt32.v len + 352 < pow2 32} -> *)
-(*   g:point{disjoint g signature} -> *)
-(*   Stack unit *)
-(*     (requires (fun h -> live h signature /\ live h msg /\ live h secret /\ live h g /\  *)
-(*       as_point h g == Spec.Ed25519.g)) *)
-(*     (ensures (fun h0 _ h1 -> live h0 signature /\ live h0 msg /\ live h0 secret /\ *)
-(*       live h1 signature /\ modifies_1 signature h0 h1 /\ *)
-(*       h1.[signature] == Spec.Ed25519.sign h0.[secret] h0.[msg])) *)
-
-(* #reset-options "--max_fuel 0 --z3rlimit 50" *)
-
-(* let sign_ signature secret msg len g = *)
-(*   push_frame(); *)
-(*   let tmp_bytes = Buffer.create 0uy (352ul +^ len) in *)
-(*   push_frame(); *)
-(*   let h0 = ST.get() in *)
-(*   let tmp_ints  = Buffer.create 0uL 65ul in *)
-(*   let msg'      = Buffer.sub tmp_bytes 64ul len in *)
-(*   let h1 = ST.get() in *)
-(*   no_upd_lemma_0 h0 h1 g; *)
-(*   no_upd_lemma_0 h0 h1 msg; *)
-(*   copy_bytes msg' msg len; *)
-(*   let h2 = ST.get() in *)
-(*   no_upd_lemma_1 h1 h2 msg' g; *)
-(*   assert(modifies_0 h0 h2); *)
-(*   sign__ signature secret msg len g tmp_bytes tmp_ints; *)
-(*   let h3 = ST.get() in *)
-(*   pop_frame(); *)
-(*   pop_frame() *)
-
-
-(* val sign: *)
-(*   signature:hint8_p{length signature = 64} -> *)
-(*   secret:hint8_p{length secret = 32} -> *)
-(*   msg:hint8_p{length msg < pow2 32 - 64} -> *)
-(*   len:UInt32.t{UInt32.v len = length msg /\ UInt32.v len + 352 < pow2 32} -> *)
-(*   Stack unit *)
-(*     (requires (fun h -> live h signature /\ live h msg /\ live h secret)) *)
-(*     (ensures (fun h0 _ h1 -> live h0 signature /\ live h0 msg /\ live h0 secret /\ *)
-(*       live h1 signature /\ modifies_1 signature h0 h1 /\ *)
-(*       h1.[signature] == Spec.Ed25519.sign h0.[secret] h0.[msg])) *)
-
-(* #reset-options "--max_fuel 0 --z3rlimit 20" *)
-
-(* let sign signature secret msg len = *)
-(*   push_frame(); *)
-(*   let h0 = ST.get() in *)
-(*   let g = create 0uL 20ul in *)
-(*   Hacl.Impl.Ed25519.G.make_g g; *)
-(*   let h1 = ST.get() in *)
-(*   assume (as_point h1 g == Spec.Ed25519.g); *)
-(*   sign_ signature secret msg len g; *)
-(*   let h2 = ST.get() in *)
-(*   pop_frame() *)
