code/experimental/ed25519/Hacl.Impl.SHA512.ModQ.fst
@@ -7,38 +7,38 @@ open Hacl.UInt64
 
 #reset-options "--max_fuel 0 --z3rlimit 20"
 
-[@ "substitute"]
-private
-val sha512_modq_:
-  out:qelemB ->
-  input:buffer Hacl.UInt8.t ->
-  len  :UInt32.t{UInt32.v len = length input} ->
-  tmp:buffer Hacl.UInt64.t{length tmp = 10 /\ disjoint out tmp} ->
-  Stack unit
-        (requires (fun h0 -> live h0 input /\ live h0 out /\ live h0 tmp))
-        (ensures  (fun h0 _ h1 -> live h0 input /\ live h1 out /\ modifies_2 out tmp h0 h1 /\
-          Hacl.Spec.BignumQ.Eval.eval_q (as_seq h1 out) == Spec.Ed25519.sha512_modq (as_seq h0 input) /\
-          (let out = as_seq h1 out in let op_String_Access = Seq.index in
-           v (out.[0]) < 0x100000000000000 /\ v (out.[1]) < 0x100000000000000 /\
-           v (out.[2]) < 0x100000000000000 /\ v (out.[3]) < 0x100000000000000 /\
-           v (out.[4]) < 0x100000000000000) ))
-#reset-options "--max_fuel 0 --z3rlimit 200"
-let sha512_modq_ out input len tmp =
-  assert_norm(pow2 32 = 0x100000000);
-  let h0 = ST.get() in
-  push_frame();
-  let hash = create (Hacl.Cast.uint8_to_sint8 0uy) 64ul in
-  Hacl.Impl.Sha512.sha512 hash input len;
-  Hacl.Impl.Load56.load_64_bytes tmp hash;
-  pop_frame();
-  let h1 = ST.get() in
-  assert(modifies_1 tmp h0 h1);
-  assert(let t = as_seq h1 tmp in Hacl.Spec.BignumQ.Mul.all_10_bellow_56 t);
-  assert(let t = as_seq h1 tmp in let op_String_Access = Seq.index in
-    Hacl.Spec.BignumQ.Eval.eval_q_10 t.[0] t.[1] t.[2] t.[3] t.[4] t.[5] t.[6] t.[7] t.[8] t.[9] < pow2 512);
-  Hacl.Impl.BignumQ.Mul.barrett_reduction out tmp;
-  assert_norm(pow2 252 + 27742317777372353535851937790883648493 =
-    0x1000000000000000000000000000000014def9dea2f79cd65812631a5cf5d3ed)
+(* [@ "substitute"] *)
+(* private *)
+(* val sha512_modq_: *)
+(*   out:qelemB -> *)
+(*   input:buffer Hacl.UInt8.t -> *)
+(*   len  :UInt32.t{UInt32.v len = length input} -> *)
+(*   tmp:buffer Hacl.UInt64.t{length tmp = 10 /\ disjoint out tmp} -> *)
+(*   Stack unit *)
+(*         (requires (fun h0 -> live h0 input /\ live h0 out /\ live h0 tmp)) *)
+(*         (ensures  (fun h0 _ h1 -> live h0 input /\ live h1 out /\ modifies_2 out tmp h0 h1 /\ *)
+(*           Hacl.Spec.BignumQ.Eval.eval_q (as_seq h1 out) == Spec.Ed25519.sha512_modq (as_seq h0 input) /\ *)
+(*           (let out = as_seq h1 out in let op_String_Access = Seq.index in *)
+(*            v (out.[0]) < 0x100000000000000 /\ v (out.[1]) < 0x100000000000000 /\ *)
+(*            v (out.[2]) < 0x100000000000000 /\ v (out.[3]) < 0x100000000000000 /\ *)
+(*            v (out.[4]) < 0x100000000000000) )) *)
+(* #reset-options "--max_fuel 0 --z3rlimit 200" *)
+(* let sha512_modq_ out input len tmp = *)
+(*   assert_norm(pow2 32 = 0x100000000); *)
+(*   let h0 = ST.get() in *)
+(*   push_frame(); *)
+(*   let hash = create (Hacl.Cast.uint8_to_sint8 0uy) 64ul in *)
+(*   Hacl.Impl.Sha512.sha512 hash input len; *)
+(*   Hacl.Impl.Load56.load_64_bytes tmp hash; *)
+(*   pop_frame(); *)
+(*   let h1 = ST.get() in *)
+(*   assert(modifies_1 tmp h0 h1); *)
+(*   assert(let t = as_seq h1 tmp in Hacl.Spec.BignumQ.Mul.all_10_bellow_56 t); *)
+(*   assert(let t = as_seq h1 tmp in let op_String_Access = Seq.index in *)
+(*     Hacl.Spec.BignumQ.Eval.eval_q_10 t.[0] t.[1] t.[2] t.[3] t.[4] t.[5] t.[6] t.[7] t.[8] t.[9] < pow2 512); *)
+(*   Hacl.Impl.BignumQ.Mul.barrett_reduction out tmp; *)
+(*   assert_norm(pow2 252 + 27742317777372353535851937790883648493 = *)
+(*     0x1000000000000000000000000000000014def9dea2f79cd65812631a5cf5d3ed) *)
 
 
 private
@@ -53,12 +53,111 @@ let lemma_modifies_0_2 #a #a' h0 h1 h2 b b' =
 
 #reset-options "--max_fuel 0 --z3rlimit 200"
 
-let sha512_modq out input len =
+(* let sha512_modq out input len = *)
+(*   push_frame(); *)
+(*   let h0 = ST.get() in *)
+(*   let tmp = create (Hacl.Cast.uint64_to_sint64 0uL) 10ul in *)
+(*   let h1 = ST.get() in *)
+(*   sha512_modq_ out input len tmp; *)
+(*   let h2 = ST.get() in *)
+(*   lemma_modifies_0_2 h0 h1 h2 out tmp; *)
+(*   pop_frame() *)
+
+
+[@ "substitute"]
+private
+val sha512_modq_pre_:
+  out:qelemB ->
+  prefix:buffer Hacl.UInt8.t{length prefix = 32} ->
+  input:buffer Hacl.UInt8.t ->
+  len  :UInt32.t{UInt32.v len = length input /\ length input < pow2 32 - 32} ->
+  tmp:buffer Hacl.UInt64.t{length tmp = 10 /\ disjoint out tmp} ->
+  Stack unit
+        (requires (fun h0 -> live h0 input /\ live h0 out /\ live h0 tmp))
+        (ensures  (fun h0 _ h1 -> live h0 input /\ live h1 out /\ modifies_2 out tmp h0 h1 /\
+          Hacl.Spec.BignumQ.Eval.eval_q (as_seq h1 out) == Spec.Ed25519.sha512_modq FStar.Seq.(as_seq h0 prefix @| as_seq h0 input) /\
+          (let out = as_seq h1 out in let op_String_Access = Seq.index in
+           v (out.[0]) < 0x100000000000000 /\ v (out.[1]) < 0x100000000000000 /\
+           v (out.[2]) < 0x100000000000000 /\ v (out.[3]) < 0x100000000000000 /\
+           v (out.[4]) < 0x100000000000000) ))
+#reset-options "--max_fuel 0 --z3rlimit 200"
+let sha512_modq_pre_ out prefix input len tmp =
+  assert_norm(pow2 32 = 0x100000000);
+  let h0 = ST.get() in
+  push_frame();
+  let hash = create (Hacl.Cast.uint8_to_sint8 0uy) 64ul in
+  Hacl.Impl.Sha512.sha512_pre_msg hash prefix input len;
+  Hacl.Impl.Load56.load_64_bytes tmp hash;
+  pop_frame();
+  let h1 = ST.get() in
+  assert(modifies_1 tmp h0 h1);
+  assert(let t = as_seq h1 tmp in Hacl.Spec.BignumQ.Mul.all_10_bellow_56 t);
+  assert(let t = as_seq h1 tmp in let op_String_Access = Seq.index in
+    Hacl.Spec.BignumQ.Eval.eval_q_10 t.[0] t.[1] t.[2] t.[3] t.[4] t.[5] t.[6] t.[7] t.[8] t.[9] < pow2 512);
+  Hacl.Impl.BignumQ.Mul.barrett_reduction out tmp;
+  assert_norm(pow2 252 + 27742317777372353535851937790883648493 =
+    0x1000000000000000000000000000000014def9dea2f79cd65812631a5cf5d3ed)
+
+
+
+#reset-options "--max_fuel 0 --z3rlimit 200"
+
+let sha512_modq_pre out prefix input len =
   push_frame();
   let h0 = ST.get() in
   let tmp = create (Hacl.Cast.uint64_to_sint64 0uL) 10ul in
   let h1 = ST.get() in
-  sha512_modq_ out input len tmp;
+  sha512_modq_pre_ out prefix input len tmp;
+  let h2 = ST.get() in
+  lemma_modifies_0_2 h0 h1 h2 out tmp;
+  pop_frame()
+
+
+[@ "substitute"]
+private
+val sha512_modq_pre_pre2_:
+  out:qelemB ->
+  prefix:buffer Hacl.UInt8.t{length prefix = 32} ->
+  prefix2:buffer Hacl.UInt8.t{length prefix2 = 32} ->
+  input:buffer Hacl.UInt8.t ->
+  len  :UInt32.t{UInt32.v len = length input /\ length input < pow2 32 - 32} ->
+  tmp:buffer Hacl.UInt64.t{length tmp = 10 /\ disjoint out tmp} ->
+  Stack unit
+        (requires (fun h0 -> live h0 input /\ live h0 out /\ live h0 tmp))
+        (ensures  (fun h0 _ h1 -> live h0 input /\ live h1 out /\ modifies_2 out tmp h0 h1 /\
+          Hacl.Spec.BignumQ.Eval.eval_q (as_seq h1 out) == Spec.Ed25519.sha512_modq FStar.Seq.(as_seq h0 prefix @| as_seq h0 prefix2 @| as_seq h0 input) /\
+          (let out = as_seq h1 out in let op_String_Access = Seq.index in
+           v (out.[0]) < 0x100000000000000 /\ v (out.[1]) < 0x100000000000000 /\
+           v (out.[2]) < 0x100000000000000 /\ v (out.[3]) < 0x100000000000000 /\
+           v (out.[4]) < 0x100000000000000) ))
+#reset-options "--max_fuel 0 --z3rlimit 200"
+let sha512_modq_pre_pre2_ out prefix prefix2 input len tmp =
+  assert_norm(pow2 32 = 0x100000000);
+  let h0 = ST.get() in
+  push_frame();
+  let hash = create (Hacl.Cast.uint8_to_sint8 0uy) 64ul in
+  Hacl.Impl.Sha512.sha512_pre_pre2_msg hash prefix prefix2 input len;
+  Hacl.Impl.Load56.load_64_bytes tmp hash;
+  pop_frame();
+  let h1 = ST.get() in
+  assert(modifies_1 tmp h0 h1);
+  assert(let t = as_seq h1 tmp in Hacl.Spec.BignumQ.Mul.all_10_bellow_56 t);
+  assert(let t = as_seq h1 tmp in let op_String_Access = Seq.index in
+    Hacl.Spec.BignumQ.Eval.eval_q_10 t.[0] t.[1] t.[2] t.[3] t.[4] t.[5] t.[6] t.[7] t.[8] t.[9] < pow2 512);
+  Hacl.Impl.BignumQ.Mul.barrett_reduction out tmp;
+  assert_norm(pow2 252 + 27742317777372353535851937790883648493 =
+    0x1000000000000000000000000000000014def9dea2f79cd65812631a5cf5d3ed)
+
+
+
+#reset-options "--max_fuel 0 --z3rlimit 200"
+
+let sha512_modq_pre_pre2 out prefix prefix2 input len =
+  push_frame();
+  let h0 = ST.get() in
+  let tmp = create (Hacl.Cast.uint64_to_sint64 0uL) 10ul in
+  let h1 = ST.get() in
+  sha512_modq_pre_pre2_ out prefix prefix2 input len tmp;
   let h2 = ST.get() in
   lemma_modifies_0_2 h0 h1 h2 out tmp;
   pop_frame()
