code/experimental/ed25519/Hacl.Impl.Sha512.fst
@@ -1,21 +1,166 @@
 module Hacl.Impl.Sha512
 
 
+open FStar.UInt32
 open FStar.Buffer
 
+open SHA2_512
 
-#reset-options "--max_fuel 0 --max_ifuel 0 --z3rlimit 20"
+
+#set-options "--lax"
 
 let hint8_p = buffer Hacl.UInt8.t
 let op_String_Access h b = Hacl.Spec.Endianness.reveal_sbytes (as_seq h b)
 
 
-assume val sha512:
-  hash :hint8_p{length hash = 64} ->
-  input:hint8_p ->
-  len  :UInt32.t{UInt32.v len = length input} ->
+val sha512_pre_msg_1:
+  hash:hint8_p{length hash = 64} ->
+  prefix:hint8_p{length prefix = 32 /\ disjoint prefix hash} ->
+  input:hint8_p{disjoint input hash} ->
+  len:UInt32.t{UInt32.v len = length input /\ length input <= 96} ->
   Stack unit
-        (requires (fun h0 -> live h0 hash /\ live h0 input))
-        (ensures  (fun h0 _ h1 -> live h0 hash /\ live h0 input /\
-          live h1 hash /\ modifies_1 hash h0 h1 /\
-          h1.[hash] == Spec.Sha512.sha512 h0.[input]))
+    (requires (fun h -> live h hash /\ live h prefix /\ live h input))
+    (ensures (fun h0 _ h1 -> live h0 hash /\ live h0 prefix /\ live h0 input /\
+      live h1 hash /\ live h1 prefix /\ live h1 input /\ modifies_1 hash h0 h1 /\
+      as_seq h1 hash == Spec.Ed25519.sha512 FStar.Seq.(as_seq h0 prefix @| as_seq h0 input)))
+
+
+let sha512_pre_msg_1 h prefix input len =
+  push_frame();
+  let block = create 0uy 128ul in
+  blit prefix 0ul block 0ul 32ul;
+  blit input 0ul block 32ul len;
+  hash h block (len +^ 32ul);
+  pop_frame()
+
+
+val sha512_pre_msg_2:
+  hash:hint8_p{length hash = 64} ->
+  prefix:hint8_p{length prefix = 32 /\ disjoint prefix hash} ->
+  input:hint8_p{disjoint input hash} ->
+  len:UInt32.t{v len = length input /\ length input > 96} ->
+  Stack unit
+    (requires (fun h -> live h hash /\ live h prefix /\ live h input))
+    (ensures (fun h0 _ h1 -> live h0 hash /\ live h0 prefix /\ live h0 input /\
+      live h1 hash /\ live h1 prefix /\ live h1 input /\ modifies_1 hash h0 h1 /\
+      as_seq h1 hash == Spec.Ed25519.sha512 FStar.Seq.(as_seq h0 prefix @| as_seq h0 input)))
+
+let sha512_pre_msg_2 h prefix input len =
+  push_frame();
+  let block = create 0uy 128ul in
+  blit prefix 0ul block 0ul 32ul;
+  blit input  0ul block 32ul 96ul;
+  let len'  = len -^ 96ul in
+  let nblocks = len' >>^ 7ul in
+  let rest    = Int.Cast.uint32_to_uint64 (len' &^ 127ul) in
+  let st      = create 0uL 169ul in
+  (* let st      = alloc () in *)
+  init st;
+  update st block;
+  update_multi st (Buffer.sub input 96ul (128ul *^ nblocks)) nblocks;
+  update_last st (Buffer.offset input (96ul +^ 128ul *^ nblocks)) rest;
+  finish st h;
+  pop_frame()
+
+
+val sha512_pre_msg:
+  hash:hint8_p{length hash = 64} ->
+  prefix:hint8_p{length prefix = 32 /\ disjoint prefix hash} ->
+  input:hint8_p{disjoint input hash} ->
+  len:UInt32.t{UInt32.v len = length input /\ length input < pow2 32 - 32} ->
+  Stack unit
+    (requires (fun h -> live h hash /\ live h prefix /\ live h input))
+    (ensures (fun h0 _ h1 -> live h0 hash /\ live h0 prefix /\ live h0 input /\
+      live h1 hash /\ live h1 prefix /\ live h1 input /\ modifies_1 hash h0 h1 /\
+      as_seq h1 hash == Spec.Ed25519.sha512 FStar.Seq.(as_seq h0 prefix @| as_seq h0 input)))
+
+
+let sha512_pre_msg h prefix input len =
+  (* push_frame(); *)
+  (* let bla = create 0uy (len +^ 32ul) in *)
+  (* blit prefix 0ul bla 0ul 32ul; *)
+  (* blit input  0ul bla 32ul len; *)
+  (* hash h bla (len +^ 32ul); *)
+  (* pop_frame() *)
+  if len <=^ 96ul then sha512_pre_msg_1 h prefix input len
+  else sha512_pre_msg_2 h prefix input len
+
+
+val sha512_pre_pre2_msg_1:
+  hash:hint8_p{length hash = 64} ->
+  prefix:hint8_p{length prefix = 32 /\ disjoint prefix hash} ->
+  prefix2:hint8_p{length prefix = 32 /\ disjoint prefix2 hash} ->
+  input:hint8_p{disjoint input hash} ->
+  len:UInt32.t{UInt32.v len = length input /\ length input <= 64} ->
+  Stack unit
+    (requires (fun h -> live h hash /\ live h prefix /\ live h input /\ live h prefix2))
+    (ensures (fun h0 _ h1 -> live h0 hash /\ live h0 prefix /\ live h0 input /\ live h0 prefix2 /\
+      live h1 hash /\ live h1 prefix /\ live h1 prefix2 /\ live h1 input /\ modifies_1 hash h0 h1 /\
+      as_seq h1 hash == Spec.Ed25519.sha512 FStar.Seq.(as_seq h0 prefix @| as_seq h0 prefix2 @| as_seq h0 input)))
+
+
+let sha512_pre_pre2_msg_1 h prefix prefix2 input len =
+  push_frame();
+  let block = create 0uy 128ul in
+  blit prefix 0ul block 0ul 32ul;
+  blit prefix2 0ul block 32ul 32ul;
+  blit input 0ul block 64ul len;
+  hash h block (len +^ 64ul);
+  pop_frame()
+
+
+val sha512_pre_pre2_msg_2:
+  hash:hint8_p{length hash = 64} ->
+  prefix:hint8_p{length prefix = 32 /\ disjoint prefix hash} ->
+  prefix2:hint8_p{length prefix = 32 /\ disjoint prefix2 hash} ->
+  input:hint8_p{disjoint input hash} ->
+  len:UInt32.t{v len = length input /\ length input > 64} ->
+  Stack unit
+    (requires (fun h -> live h hash /\ live h prefix /\ live h prefix2 /\ live h input))
+    (ensures (fun h0 _ h1 -> live h0 hash /\ live h0 prefix /\ live h0 prefix2 /\ live h0 input /\
+      live h1 hash /\ live h1 prefix /\ live h1 prefix2 /\ live h1 input /\ modifies_1 hash h0 h1 /\
+      as_seq h1 hash == Spec.Ed25519.sha512 FStar.Seq.(as_seq h0 prefix @| as_seq h0 prefix2 @| as_seq h0 input)))
+
+
+let sha512_pre_pre2_msg_2 h prefix prefix2 input len =
+  push_frame();
+  let block = create 0uy 128ul in
+  blit prefix 0ul block 0ul 32ul;
+  blit prefix2 0ul block 32ul 32ul;
+  blit input 0ul block 64ul 64ul;
+  let len'  = len -^ 64ul in
+  let nblocks = len' >>^ 7ul in
+  let rest    = Int.Cast.uint32_to_uint64 (len' &^ 127ul) in
+  let st      = create 0uL 169ul in
+  init st;
+  update st block;
+  update_multi st (Buffer.sub input 64ul (128ul *^ nblocks)) nblocks;
+  update_last st (Buffer.offset input (64ul +^ 128ul *^ nblocks)) rest;
+  finish st h;
+  pop_frame()
+
+
+
+val sha512_pre_pre2_msg:
+  hash:hint8_p{length hash = 64} ->
+  prefix:hint8_p{length prefix = 32 /\ disjoint prefix hash} ->
+  prefix2:hint8_p{length prefix = 32 /\ disjoint prefix2 hash} ->
+  input:hint8_p{disjoint input hash} ->
+  len:UInt32.t{UInt32.v len = length input /\ length input < pow2 32 - 64} ->
+  Stack unit
+    (requires (fun h -> live h hash /\ live h prefix /\ live h prefix2 /\ live h input))
+    (ensures (fun h0 _ h1 -> live h0 hash /\ live h0 prefix /\ live h0 input /\
+      live h1 hash /\ live h1 prefix /\ live h1 input /\ modifies_1 hash h0 h1 /\
+      as_seq h1 hash == Spec.Ed25519.sha512 FStar.Seq.(as_seq h0 prefix @| as_seq h0 prefix2 @| as_seq h0 input)))
+
+
+let sha512_pre_pre2_msg h prefix prefix2 input len =
+  (* push_frame(); *)
+  (* let bla = create 0uy (len +^ 64ul) in *)
+  (* blit prefix  0ul bla 0ul 32ul; *)
+  (* blit prefix2 0ul bla 32ul 32ul; *)
+  (* blit input   0ul bla 64ul len; *)
+  (* hash h bla (len +^ 64ul); *)
+  (* pop_frame() *)
+  if len <=^ 64ul then sha512_pre_pre2_msg_1 h prefix prefix2 input len
+  else sha512_pre_pre2_msg_2 h prefix prefix2 input len
