code/experimental/hash/SHA2_512.fst
@@ -30,20 +30,6 @@ module Spec = Spec.SHA2_512
 module Hash = Hacl.Hash.SHA2_512
 
 
-(* Definition of base types *)
-private let uint8_t   = FStar.UInt8.t
-private let uint32_t  = FStar.UInt32.t
-private let uint64_t  = FStar.UInt64.t
-
-private let uint8_ht  = Hacl.UInt8.t
-private let uint32_ht = Hacl.UInt32.t
-private let uint64_ht = Hacl.UInt64.t
-private let uint128_ht = Hacl.UInt128.t
-
-private let uint64_p = Buffer.buffer uint64_ht
-private let uint8_p  = Buffer.buffer uint8_ht
-
-
 (* Definitions of aliases for functions *)
 private let u8_to_h8 = Cast.uint8_to_sint8
 private let u32_to_h32 = Cast.uint32_to_sint32
@@ -70,163 +56,29 @@ private let h64_to_h128 = Cast.sint64_to_sint128
 //
 // SHA-512
 //
-(* Define algorithm parameters *)
-let size_hash = Hash.size_hash
-let size_block = Hash.size_block
-let size_state = Hash.size_state
-
-
-[@"c_inline"]
-val alloc:
-  unit ->
-  StackInline (state:uint64_p{length state = v size_state})
-    (requires (fun h0 -> True))
-    (ensures (fun h0 st h1 -> ~(contains h0 st) /\ live h1 st /\ modifies_0 h0 h1 /\ frameOf st == h1.tip
-             /\ Map.domain h1.h == Map.domain h0.h))
 
 #reset-options "--max_fuel 0  --z3rlimit 50"
 
 [@"c_inline"]
 let alloc () = alloc ()
 
-
-#reset-options "--max_fuel 0  --z3rlimit 50"
-
-val init:
-  state:uint64_p{length state = v size_state} ->
-  Stack unit
-    (requires (fun h0 -> live h0 state
-              /\ (let seq_counter = Seq.slice (as_seq h0 state) (U32.v pos_count_w) (U32.(v pos_count_w + v size_count_w)) in
-              let counter = Seq.index seq_counter 0 in
-              H64.v counter = 0)))
-    (ensures  (fun h0 r h1 -> live h1 state /\ modifies_1 state h0 h1
-              /\ (let slice_k = Seq.slice (as_seq h1 state) (U32.v pos_k_w) (U32.(v pos_k_w + v size_k_w)) in
-              let slice_h_0 = Seq.slice (as_seq h1 state) (U32.v pos_whash_w) (U32.(v pos_whash_w + v size_whash_w)) in
-              let seq_counter = Seq.slice (as_seq h1 state) (U32.v pos_count_w) (U32.(v pos_count_w + v size_count_w)) in
-              let counter = Seq.index seq_counter 0 in
-              let seq_k = Hacl.Spec.Endianness.reveal_h64s slice_k in
-              let seq_h_0 = Hacl.Spec.Endianness.reveal_h64s slice_h_0 in
-              seq_k == Spec.k /\ seq_h_0 == Spec.h_0 /\ H64.v counter = 0)))
-
 #reset-options "--max_fuel 0  --z3rlimit 50"
 
 let init state = init state
-
-
-#reset-options "--max_fuel 0  --z3rlimit 50"
-
-val update:
-  state :uint64_p {length state = v size_state} ->
-  data  :uint8_p  {length data = v size_block /\ disjoint state data} ->
-  Stack unit
-        (requires (fun h0 -> live h0 state /\ live h0 data
-                  /\ (let seq_k = Seq.slice (as_seq h0 state) (U32.v pos_k_w) (U32.(v pos_k_w + v size_k_w)) in
-                  let seq_counter = Seq.slice (as_seq h0 state) (U32.v pos_count_w) (U32.(v pos_count_w + v size_count_w)) in
-                  let counter = Seq.index seq_counter 0 in
-                  seq_k == Spec.k /\ H64.v counter < (pow2 64 - 1))))
-        (ensures  (fun h0 r h1 -> live h0 state /\ live h0 data /\ live h1 state /\ modifies_1 state h0 h1
-                  /\ (let seq_hash_0 = Seq.slice (as_seq h0 state) (U32.v pos_whash_w) (U32.(v pos_whash_w + v size_whash_w)) in
-                  let seq_hash_1 = Seq.slice (as_seq h1 state) (U32.v pos_whash_w) (U32.(v pos_whash_w + v size_whash_w)) in
-                  let seq_k_0 = Seq.slice (as_seq h0 state) (U32.v pos_k_w) (U32.(v pos_k_w + v size_k_w)) in
-                  let seq_k_1 = Seq.slice (as_seq h1 state) (U32.v pos_k_w) (U32.(v pos_k_w + v size_k_w)) in
-                  let seq_block = as_seq h0 data in
-                  let seq_counter_0 = Seq.slice (as_seq h0 state) (U32.v pos_count_w) (U32.(v pos_count_w + v size_count_w)) in
-                  let seq_counter_1 = Seq.slice (as_seq h1 state) (U32.v pos_count_w) (U32.(v pos_count_w + v size_count_w)) in
-                  let counter_0 = Seq.index seq_counter_0 0 in
-                  let counter_1 = Seq.index seq_counter_1 0 in
-                  seq_k_0 == seq_k_1
-                  /\ H64.v counter_1 = H64.v counter_0 + 1 /\ H64.v counter_1 < pow2 64
-                  /\ seq_hash_1 == Spec.update seq_hash_0 seq_block)))
 
 #reset-options "--max_fuel 0  --z3rlimit 200"
 
 let update state data = update state data
 
-
-#reset-options "--max_fuel 0  --z3rlimit 100"
-
-val update_multi:
-  state :uint64_p{length state = v size_state} ->
-  data  :uint8_p {length data % v size_block = 0 /\ disjoint state data} ->
-  n     :uint32_t{v n * v size_block = length data} ->
-  Stack unit
-        (requires (fun h0 -> live h0 state /\ live h0 data
-                  /\ (let seq_k = Seq.slice (as_seq h0 state) (U32.v pos_k_w) (U32.(v pos_k_w + v size_k_w)) in
-                  let seq_counter = Seq.slice (as_seq h0 state) (U32.v pos_count_w) (U32.(v pos_count_w + v size_count_w)) in
-                  let counter = Seq.index seq_counter 0 in
-                  seq_k == Spec.k /\ H64.v counter < (pow2 64 - (v n)))))
-        (ensures  (fun h0 _ h1 -> live h0 state /\ live h0 data /\ live h1 state /\ modifies_1 state h0 h1
-                  /\ (let seq_hash_0 = Seq.slice (as_seq h0 state) (U32.v pos_whash_w) (U32.(v pos_whash_w + v size_whash_w)) in
-                  let seq_hash_1 = Seq.slice (as_seq h1 state) (U32.v pos_whash_w) (U32.(v pos_whash_w + v size_whash_w)) in
-                  let seq_k_0 = Seq.slice (as_seq h0 state) (U32.v pos_k_w) (U32.(v pos_k_w + v size_k_w)) in
-                  let seq_k_1 = Seq.slice (as_seq h1 state) (U32.v pos_k_w) (U32.(v pos_k_w + v size_k_w)) in
-                  let seq_blocks = as_seq h0 data in
-                  let seq_counter_0 = Seq.slice (as_seq h0 state) (U32.v pos_count_w) (U32.(v pos_count_w + v size_count_w)) in
-                  let seq_counter_1 = Seq.slice (as_seq h1 state) (U32.v pos_count_w) (U32.(v pos_count_w + v size_count_w)) in
-                  let counter_0 = Seq.index seq_counter_0 0 in
-                  let counter_1 = Seq.index seq_counter_1 0 in
-                  seq_k_0 == seq_k_1
-                  /\ H64.v counter_1 = H64.v counter_0 + (v n) /\ H64.v counter_1 < pow2 64
-                  /\ seq_hash_1 == Spec.update_multi seq_hash_0 seq_blocks)))
-
 #reset-options "--max_fuel 0  --z3rlimit 200"
 
 let rec update_multi state data n = update_multi state data n
-
-
-#reset-options "--max_fuel 0  --z3rlimit 50"
-
-val update_last:
-  state :uint64_p {length state = v size_state} ->
-  data  :uint8_p  {disjoint state data} ->
-  len   :uint64_t {U64.v len = length data /\ (length data + v size_len_8 + 1) < 2 * v size_block} ->
-  Stack unit
-        (requires (fun h0 -> live h0 state /\ live h0 data
-                  /\ (let seq_k = Seq.slice (as_seq h0 state) (U32.v pos_k_w) (U32.(v pos_k_w + v size_k_w)) in
-                  let seq_counter = Seq.slice (as_seq h0 state) (U32.v pos_count_w) (U32.(v pos_count_w + v size_count_w)) in
-                  let counter = Seq.index seq_counter 0 in
-                  let nb = U64.div len (u32_to_u64 size_block) in
-                  seq_k == Spec.k /\ H64.v counter < (pow2 64 - 2))))
-        (ensures  (fun h0 r h1 -> live h0 state /\ live h0 data /\ live h1 state /\ modifies_1 state h0 h1
-                  /\ (let seq_hash_0 = Seq.slice (as_seq h0 state) (U32.v pos_whash_w) (U32.(v pos_whash_w + v size_whash_w)) in
-                  let seq_hash_1 = Seq.slice (as_seq h1 state) (U32.v pos_whash_w) (U32.(v pos_whash_w + v size_whash_w)) in
-                  let seq_data = as_seq h0 data in
-                  let count = Seq.slice (as_seq h0 state) (U32.v pos_count_w) (U32.v pos_count_w + 1) in
-                  let prevlen = U64.(v (Seq.index count 0) * (U32.v size_block)) in
-                  seq_hash_1 == Spec.update_last seq_hash_0 prevlen seq_data)))
 
 #reset-options "--max_fuel 0  --z3rlimit 200"
 
 let update_last state data len = update_last state data len
 
-
-#reset-options "--max_fuel 0  --z3rlimit 10"
-
-val finish:
-  state :uint64_p{length state = v size_state} ->
-  hash  :uint8_p{length hash = v size_hash} ->
-  Stack unit
-        (requires (fun h0 -> live h0 state /\ live h0 hash))
-        (ensures  (fun h0 _ h1 -> live h0 state /\ live h1 hash /\ modifies_1 hash h0 h1
-                  /\ (let seq_hash_w = Seq.slice (as_seq h0 state) (U32.v pos_whash_w) (U32.(v pos_whash_w + v size_whash_w)) in
-                  let seq_hash = as_seq h1 hash in
-                  seq_hash = Spec.finish seq_hash_w)))
-
 let finish state hash = finish state hash
-
-
-#reset-options "--max_fuel 0  --z3rlimit 10"
-
-val hash:
-  hash :uint8_p {length hash = v size_hash} ->
-  input:uint8_p {length input < Spec.max_input_len_8} ->
-  len  :uint32_t{v len = length input} ->
-  Stack unit
-        (requires (fun h0 -> live h0 hash /\ live h0 input))
-        (ensures  (fun h0 _ h1 -> live h0 input /\ live h0 hash /\ live h1 hash /\ modifies_1 hash h0 h1
-                  /\ (let seq_input = as_seq h0 input in
-                  let seq_hash = as_seq h1 hash in
-                  seq_hash == Spec.hash seq_input)))
 
 #reset-options "--max_fuel 0  --z3rlimit 50"
 
